veric/binop_lemmas.v
@@ -27,31 +27,25 @@ extensionality a rho.
 destruct a; reflexivity.
 Qed.
 
-Ltac typecheck_sound_solver1 H0 e1 e2 t :=
-rewrite <- denote_tc_assert'_eq in *;
-simpl in *;
- destruct (typeof e1) as [ | [ | | | ] [ | ]  | [ | ]  | | | | | | ]; 
-      try (contradiction H0);
- destruct (typeof e2) as [ | [ | | | ] [ | ]  | [ | ]  | | | | | | ]; 
-      try (contradiction H0);
- destruct t; try (contradiction H0);
-simpl in *.
-
-Lemma cmp_sound_aux:
-  forall b i s a , typecheck_val (force_val (Some (Val.of_bool b))) (Tint i s a) = true.
-Proof. destruct b; reflexivity. Qed.
- 
 Lemma int_eq_true : forall x y,
 true = Int.eq x y -> x = y.
 Proof.
 intros. assert (X := Int.eq_spec x y). if_tac in X; auto. congruence.
 Qed.
 
-Definition check_pp_int' e1 e2 op t :=
+Definition check_pp_int' e1 e2 op t e :=
 match op with 
-| Cop.Oeq | Cop.One => tc_andp 
-                         (tc_orp (tc_iszero' e1) (tc_iszero' e2))
-                         (tc_bool (is_int_type t) (pp_compare_size_0 t))
+| Cop.Oeq | Cop.One => tc_andp'
+                         (tc_orp' (tc_iszero' e1) (tc_iszero' e2))
+                         (tc_bool (is_int_type t) (op_result_type e))
+| _ => tc_noproof
+end.
+
+Definition check_pl_long' e2 op t e :=
+match op with 
+| Cop.Oeq | Cop.One => tc_andp'
+                         (tc_iszero' e2)
+                         (tc_bool (is_int_type t) (op_result_type e))
 | _ => tc_noproof
 end.
 
@@ -62,24 +56,37 @@ Proof. intros; unfold tc_andp.  destruct e; reflexivity. Qed.
 Lemma tc_andp_TT1:  forall e, tc_andp tc_TT e = e. 
 Proof. intros; unfold tc_andp; reflexivity. Qed.
 
+Lemma or_False: forall x, (x \/ False) = x.
+Proof.
+intros; apply prop_ext; intuition.
+Qed.
+
+Lemma or_True: forall x, (x \/ True) = True.
+Proof.
+intros; apply prop_ext; intuition.
+Qed.
+
+Lemma True_or: forall x, (True \/ x) = True.
+Proof.
+intros; apply prop_ext; intuition.
+Qed.
+
+Lemma False_or: forall x, (False \/ x) = x.
+Proof.
+intros; apply prop_ext; intuition.
+Qed.
+
 Lemma denote_tc_assert_orp: forall x y rho, 
   denote_tc_assert (tc_orp x y) rho = (denote_tc_assert x rho \/ denote_tc_assert y rho).
 Proof.
  intros.
  unfold tc_orp.
- unfold denote_tc_assert;
- destruct x,y; simpl; auto;
- try solve [unfold_lift; simpl; apply prop_ext; intuition].
-Qed. 
-
-Lemma denote_tc_assert_andp: forall x y rho, 
-  denote_tc_assert (tc_andp x y) rho = (denote_tc_assert x rho /\ denote_tc_assert y rho).
-Proof.
- intros.
- unfold tc_andp.
- unfold denote_tc_assert;
- destruct x,y; simpl; auto;
- unfold_lift; simpl; apply prop_ext; intuition.
+ destruct x; simpl;
+  unfold_lift; simpl; try rewrite True_or; try rewrite False_or; try reflexivity;
+  destruct y; simpl; unfold_lift; simpl;
+       try rewrite True_or; try rewrite False_or; 
+       try rewrite or_True; try rewrite or_False; 
+  try reflexivity.
 Qed. 
 
 Lemma is_true_true: is_true true = True.
@@ -87,9 +94,160 @@ Proof. apply prop_ext; intuition. Qed.
 Lemma is_true_false: is_true false = False.
 Proof. apply prop_ext; intuition. Qed.
 
-Lemma and_False: forall x, (x /\ False) = False.
+
+Lemma denote_tc_assert_iszero: forall e rho,
+  denote_tc_assert (tc_iszero e) rho = 
+  match (eval_expr e rho) with 
+  | Vint i => is_true (Int.eq i Int.zero) 
+  | Vlong i => is_true (Int.eq (Int.repr (Int64.unsigned i)) Int.zero)
+   | _ => False end.
 Proof.
-intros; apply prop_ext; intuition.
+ unfold tc_iszero.
+ destruct e; simpl; intros; auto;
+ unfold_lift; simpl; 
+  try (destruct (Int.eq i Int.zero); simpl;  symmetry; try apply is_true_true; try apply is_true_false).
+ destruct ( Int.eq (Int.repr (Int64.unsigned i)) Int.zero);
+symmetry; try apply is_true_true; try apply is_true_false.
+Qed.
+
+Lemma denote_tc_assert_iszero': forall e,
+  denote_tc_assert (tc_iszero e) = denote_tc_assert (tc_iszero' e).
+Proof.
+intros.
+extensionality rho.
+rewrite denote_tc_assert_iszero.
+reflexivity.
+Qed.
+
+
+Lemma denote_tc_assert_andp'': 
+  forall a b rho, denote_tc_assert (tc_andp' a b) rho =
+             (denote_tc_assert a rho /\ denote_tc_assert b rho).
+Proof.
+ intros. reflexivity. Qed.
+
+Lemma denote_tc_assert_orp'': 
+  forall a b rho, denote_tc_assert (tc_orp' a b) rho =
+             (denote_tc_assert a rho \/ denote_tc_assert b rho).
+Proof.
+ intros. reflexivity. Qed.
+
+Lemma denote_tc_assert_andp: 
+  forall a b rho, denote_tc_assert (tc_andp a b) rho =
+             (denote_tc_assert a rho /\ denote_tc_assert b rho).
+Proof.
+ intros. apply prop_ext. rewrite tc_andp_sound.
+ simpl; apply iff_refl.
+Qed.
+
+
+Lemma denote_tc_assert_andp': 
+  forall a b, denote_tc_assert (tc_andp a b) =
+                        denote_tc_assert (tc_andp' a b).
+Proof. intros. extensionality rho. apply denote_tc_assert_andp. Qed.
+
+Lemma denote_tc_assert_orp': 
+  forall a b, denote_tc_assert (tc_orp a b) =
+                        denote_tc_assert (tc_orp' a b).
+Proof. intros. extensionality rho. apply denote_tc_assert_orp. Qed.
+
+Hint Rewrite denote_tc_assert_andp' denote_tc_assert_andp''
+    denote_tc_assert_orp' denote_tc_assert_orp''
+    denote_tc_assert_iszero' : dtca.
+
+Ltac dtca := autorewrite with dtca; auto.
+
+Definition stupid_typeconv ty := 
+match ty with
+| Tarray t _ a => Tpointer t a
+| Tfunction _ _ => Tpointer ty noattr
+| _ => ty
+end.
+
+Definition classify_sub' ty1 ty2 := 
+match stupid_typeconv ty1 with
+| Tpointer ty a =>
+    match stupid_typeconv ty2 with
+    | Tint _ _ _ => sub_case_pi ty a
+    | Tlong _ _ => sub_case_pl ty a
+    | Tpointer _ _ => sub_case_pp ty
+    | _ => sub_default
+    end
+| _ => sub_default
+end.
+
+Lemma classify_sub_eq : classify_sub = classify_sub'.
+Proof.
+unfold classify_sub, classify_sub'; extensionality t1 t2.
+destruct t1,t2; simpl; auto;
+try destruct i,s; auto;
+try destruct i0,s0; auto.
+Qed.
+
+Definition classify_cmp' ty1 ty2 := 
+  match stupid_typeconv ty1, stupid_typeconv ty2 with 
+  | Tpointer _ _ , Tpointer _ _ => cmp_case_pp
+  | Tpointer _ _ , Tint _ _ _ => cmp_case_pp
+  | Tint _ _ _, Tpointer _ _ => cmp_case_pp
+  | Tpointer _ _ , Tlong _ _ => cmp_case_pl
+  | Tlong _ _ , Tpointer _ _ => cmp_case_lp
+  | _, _ => cmp_default
+  end.
+
+Lemma classify_cmp_eq: classify_cmp = classify_cmp'.
+Proof.
+unfold classify_cmp, classify_cmp'; extensionality t1 t2.
+destruct t1,t2; simpl; auto;
+try destruct i,s; auto;
+try destruct i0,s0; auto.
+Qed.
+
+Definition classify_add' ty1 ty2 := 
+ match stupid_typeconv ty1 with
+ | Tint _ _ _ =>
+    match stupid_typeconv ty2 with
+    | Tpointer ty a => add_case_ip ty a
+    |  _ => add_default
+    end
+| Tlong _ _ =>
+    match stupid_typeconv ty2 with
+    | Tpointer ty a => add_case_lp ty a
+    | _ => add_default
+    end
+| Tpointer ty a =>
+    match stupid_typeconv ty2 with
+    | Tint _ _ _ => add_case_pi ty a
+    | Tlong _ _ => add_case_pl ty a
+    | _ => add_default
+    end
+ | _ => add_default
+end.
+
+Lemma classify_add_eq:  classify_add = classify_add'.
+Proof.
+unfold classify_add; extensionality t1 t2.
+destruct t1,t2; simpl; auto;
+try destruct i,s; auto;
+try destruct i0,s0; auto.
+Qed.
+
+Definition classify_shift' (ty1: type) (ty2: type) :=
+  match stupid_typeconv ty1, stupid_typeconv ty2 with
+  | Tint I32 Unsigned _, Tint _ _ _ => shift_case_ii Unsigned
+  | Tint _ _ _, Tint _ _ _ => shift_case_ii Signed
+  | Tint I32 Unsigned _, Tlong _ _ => shift_case_il Unsigned
+  | Tint _ _ _, Tlong _ _ => shift_case_il Signed
+  | Tlong s _, Tint _ _ _ => shift_case_li s
+  | Tlong s _, Tlong _ _ => shift_case_ll s
+  | _,_  => shift_default
+  end.
+
+Lemma classify_shift_eq:  classify_shift = classify_shift'.
+Proof.
+unfold classify_shift; extensionality t1 t2.
+destruct t1,t2; simpl; auto;
+try destruct i,s; auto;
+try destruct i0,s0; auto.
 Qed.
 
 Lemma den_isBinOpR: forall op a1 a2 ty,
@@ -97,233 +255,362 @@ Lemma den_isBinOpR: forall op a1 a2 ty,
 let e := (Ebinop op a1 a2 ty) in
 let reterr := op_result_type e in
 let deferr := arg_type e in 
- denote_tc_assert
- match op with
-  | Cop.Oadd => match Cop.classify_add (typeof a1) (typeof a2) with 
-                    | Cop.add_default => tc_FF deferr 
-                    | Cop.add_case_ii _ => tc_bool (is_int_type ty) reterr
-                    | Cop.add_case_pi _ _ => tc_andp (tc_isptr a1) (tc_bool (is_pointer_type ty) reterr ) 
-                    | Cop.add_case_ip _ _ => tc_andp (tc_isptr a2) (tc_bool (is_pointer_type ty) reterr )
-                    | _ => tc_bool (is_float_type ty) deferr 
+denote_tc_assert
+match op with
+  | Cop.Oadd => match classify_add' (typeof a1) (typeof a2) with 
+                    | Cop.add_case_pi _ _ => tc_andp' (tc_isptr a1) (tc_bool (is_pointer_type ty) reterr) 
+                    | Cop.add_case_ip _ _ => tc_andp' (tc_isptr a2) (tc_bool (is_pointer_type ty) reterr)
+                    | Cop.add_case_pl _ _ => tc_andp' (tc_isptr a1) (tc_bool (is_pointer_type ty) reterr) 
+                    | Cop.add_case_lp _ _ => tc_andp' (tc_isptr a2) (tc_bool (is_pointer_type ty) reterr)
+                    | Cop.add_default => binarithType (typeof a1) (typeof a2) ty deferr reterr
             end
-  | Cop.Osub => match Cop.classify_sub (typeof a1) (typeof a2) with 
-                    | Cop.sub_default => tc_FF deferr 
-                    | Cop.sub_case_ii _ => tc_bool (is_int_type ty) reterr 
-                    | Cop.sub_case_pi _ => tc_andp (tc_isptr a1) (tc_bool (is_pointer_type ty) reterr )
+  | Cop.Osub => match classify_sub' (typeof a1) (typeof a2) with 
+                    | Cop.sub_case_pi _ _ => tc_andp' (tc_isptr a1) (tc_bool (is_pointer_type ty) reterr)
+                    | Cop.sub_case_pl _ _ => tc_andp' (tc_isptr a1) (tc_bool (is_pointer_type ty) reterr)
                     | Cop.sub_case_pp ty2 =>  (*tc_isptr may be redundant here*)
-                             tc_andp (tc_andp (tc_andp (tc_andp (tc_samebase a1 a2)
-                             (tc_isptr a1)) (tc_isptr a2)) (tc_bool (is_int_type ty) reterr ))
-			     (tc_bool (negb (Int.eq (Int.repr (sizeof ty2)) Int.zero)) (pp_compare_size_0 ty2))
-                    | _ => tc_bool (is_float_type ty)deferr 
+                             tc_andp' (tc_andp' (tc_andp' (tc_andp' (tc_samebase a1 a2)
+                             (tc_isptr a1)) (tc_isptr a2)) (tc_bool (is_int_type ty) reterr))
+			     (tc_bool (negb (Int.eq (Int.repr (sizeof ty2)) Int.zero)) 
+                                      (pp_compare_size_0 ty2) )
+                    | Cop.sub_default => binarithType (typeof a1) (typeof a2) ty deferr reterr
             end 
-  | Cop.Omul => match Cop.classify_mul (typeof a1) (typeof a2) with 
-                    | Cop.mul_default => tc_FF deferr 
-                    | Cop.mul_case_ii _ => tc_bool (is_int_type ty) reterr 
-                    | _ => tc_bool (is_float_type ty) deferr 
-            end 
-  | Cop.Omod => match Cop.classify_binint (typeof a1) (typeof a2) with
-                    | Cop.binint_case_ii Unsigned => 
-                           tc_andp (tc_nonzero a2) 
-                           (tc_bool (is_int_type ty) reterr )
-                    | Cop.binint_case_ii Signed => tc_andp (tc_andp (tc_nonzero a2) 
+  | Cop.Omul => binarithType (typeof a1) (typeof a2) ty deferr reterr
+  | Cop.Omod => match Cop.classify_binarith (typeof a1) (typeof a2) with
+                    | Cop.bin_case_i Unsigned => 
+                           tc_andp' (tc_nonzero a2) 
+                           (tc_bool (is_int_type ty) reterr)
+                    | Cop.bin_case_l Unsigned => 
+                           tc_andp' (tc_nonzero a2) 
+                           (tc_bool (is_long_type ty) reterr)
+                    | Cop.bin_case_i Signed => tc_andp' (tc_andp' (tc_nonzero a2) 
                                                       (tc_nodivover a1 a2))
-                                                     (tc_bool (is_int_type ty) reterr )
-                    | Cop.binint_default => tc_FF deferr 
+                                                     (tc_bool (is_int_type ty) reterr)
+                    | Cop.bin_case_l Signed => tc_andp' (tc_andp' (tc_nonzero a2) 
+                                                      (tc_nodivover a1 a2))
+                                                     (tc_bool (is_long_type ty) reterr)
+                    | _ => tc_FF deferr
             end
-  | Cop.Odiv => match Cop.classify_div (typeof a1) (typeof a2) with
-                    | Cop.div_case_ii Unsigned => tc_andp (tc_nonzero a2) (tc_bool (is_int_type ty) reterr )
-                    | Cop.div_case_ii Signed => tc_andp (tc_andp (tc_nonzero a2) (tc_nodivover a1 a2)) (tc_bool (is_int_type ty) reterr )
-                    | Cop.div_case_ff | Cop.div_case_if _ | Cop.div_case_fi _ =>
-                          tc_bool (is_float_type ty) reterr 
-                    | Cop.div_default => tc_FF deferr 
+  | Cop.Odiv => match Cop.classify_binarith (typeof a1) (typeof a2) with
+                    | Cop.bin_case_i Unsigned => tc_andp' (tc_nonzero a2) (tc_bool (is_int_type ty) reterr)
+                    | Cop.bin_case_l Unsigned => tc_andp' (tc_nonzero a2) (tc_bool (is_long_type ty) reterr)
+                    | Cop.bin_case_i Signed => tc_andp' (tc_andp' (tc_nonzero a2) (tc_nodivover a1 a2)) 
+                                                        (tc_bool (is_int_type ty) reterr)
+                    | Cop.bin_case_l Signed => tc_andp' (tc_andp' (tc_nonzero a2) (tc_nodivover a1 a2)) 
+                                                        (tc_bool (is_long_type ty) reterr)
+                    | Cop.bin_case_f  =>  tc_bool (is_float_type ty) reterr 
+                    | Cop.bin_default => tc_FF deferr
             end
-  | Cop.Oshl | Cop.Oshr => match Cop.classify_shift (typeof a1) (typeof a2) with
-                    | Cop.shift_case_ii _ =>  tc_andp (tc_ilt a2 Int.iwordsize) (tc_bool (is_int_type ty) reterr )
-                    | _ => tc_FF deferr 
+  | Cop.Oshl | Cop.Oshr => match classify_shift' (typeof a1) (typeof a2) with
+                    | Cop.shift_case_ii _ =>  tc_andp' (tc_ilt a2 Int.iwordsize) (tc_bool (is_int_type ty) 
+                                                                                         reterr)
+                    | _ => tc_FF deferr
                    end
   | Cop.Oand | Cop.Oor | Cop.Oxor => 
-                   match Cop.classify_binint (typeof a1) (typeof a2) with
-                    | Cop.binint_case_ii _ =>tc_bool (is_int_type ty) reterr 
-                    | _ => tc_FF deferr 
+                   match Cop.classify_binarith (typeof a1) (typeof a2) with
+                    | Cop.bin_case_i _ =>tc_bool (is_int_type ty) reterr
+                    | _ => tc_FF deferr
                    end   
   | Cop.Oeq | Cop.One | Cop.Olt | Cop.Ogt | Cop.Ole | Cop.Oge => 
-                   match Cop.classify_cmp (typeof a1) (typeof a2) with
-                    | Cop.cmp_default => tc_FF deferr 
-		    | Cop.cmp_case_pp => check_pp_int' a1 a2 op ty
-                    | _ => tc_bool (is_int_type ty) reterr 
+                   match classify_cmp' (typeof a1) (typeof a2) with
+                    | Cop.cmp_default => 
+                           tc_bool (is_numeric_type (typeof a1) 
+                                         && is_numeric_type (typeof a2)
+                                          && is_int_type ty)
+                                             deferr
+		    | Cop.cmp_case_pp => check_pp_int' a1 a2 op ty e
+                    | Cop.cmp_case_pl => check_pl_long' a2 op ty e
+                    | Cop.cmp_case_lp => check_pl_long' a1 op ty e
                    end
   end.
 Proof.
  intros.
- unfold isBinOpResultType, classify_cmp;  destruct op; auto;
- unfold check_pp_int';
+ rewrite <- classify_add_eq. rewrite <- classify_sub_eq.
+ rewrite <- classify_shift_eq. rewrite <- classify_cmp_eq.
+ unfold isBinOpResultType, classify_add, classify_sub, classify_binarith, classify_shift, 
+  classify_cmp, check_pp_int, check_pp_int', check_pl_long, check_pl_long', typeconv;
+  destruct op; dtca;
  extensionality rho;
- destruct (typeof a1), (typeof a2); simpl; auto;
- try (destruct i; auto; destruct s; auto;
-       try (destruct i0; auto; destruct s0; auto));
- unfold_lift; unfold tc_iszero;  
-   destruct (is_int_type ty); simpl; unfold_lift; auto;
-  try rewrite tc_andp_TT2;
- repeat rewrite denote_tc_assert_andp;
- repeat rewrite denote_tc_assert_orp;
- repeat rewrite and_False;
- simpl; unfold_lift; simpl; f_equal; auto;
- unfold denote_tc_iszero;
- clear;
- repeat (match goal with a: expr |- _ => destruct a; simpl; auto end);
- try solve [unfold_lift; simpl; destruct (Int.eq i Int.zero); simpl;  symmetry; try apply is_true_true; try apply is_true_false].
+ destruct (typeof a1), (typeof a2); dtca;
+ try (destruct i; dtca); 
+ try (destruct s; dtca);
+ try (destruct i0; dtca);
+ try (destruct s0; dtca).
 Qed.
 
-(*
-Lemma check_pp_int_sound : forall e1 e2 t op rho, 
-denote_tc_assert' (check_pp_int e1 e2 op t) rho ->
-is_int_type t = true /\ 
-((exists tt, e1 = Econst_int Int.zero tt) \/
-(exists tt, e2 = Econst_int Int.zero tt)).
+Lemma denote_tc_assert'_andp'_e:
+ forall a b rho, denote_tc_assert' (tc_andp' a b) rho ->
+    denote_tc_assert' a rho /\ denote_tc_assert' b rho.
+Proof. intros.
+ rewrite denote_tc_assert'_eq in *. apply H.
+Qed.
+
+Lemma cast_int_long_nonzero:
+  forall s i, Int.eq i Int.zero = false -> 
+             Int64.eq (cast_int_long s i) Int64.zero = false.
 Proof.
 intros.
-unfold check_pp_int in *.
-destruct op; simpl in H; try inv H;
-destruct e1; simpl in H; try inv H;
-destruct e2; simpl in H; try inv H; 
-try (unfold tc_bool in H; 
-          try remember (Int.eq i Int.zero); 
-          try remember (Int.eq i0 Int.zero);
-          repeat if_tac in H; simpl in H;
-          try (contradiction H);
-          try (apply int_eq_true in Heqb);
-          try (apply int_eq_true in Heqb0);
-          subst;
-split;  eauto). 
-Qed.
-*)
+pose proof (Int.eq_spec i Int.zero). rewrite H in H0. clear H.
+rewrite Int64.eq_false; auto.
+unfold cast_int_long.
+contradict H0.
+unfold Int64.zero in H0.
+destruct s.
+assert (Int64.signed (Int64.repr (Int.signed i)) = Int64.signed (Int64.repr 0)) by (f_equal; auto).
+rewrite Int64.signed_repr in H.
+rewrite Int64.signed_repr in H.
+rewrite <- (Int.repr_signed i).
+rewrite H. reflexivity.
+pose proof (Int64.signed_range Int64.zero).
+rewrite Int64.signed_zero in H1.
+auto.
+pose proof (Int.signed_range i).
+clear - H1.
+destruct H1.
+split.
+apply Z.le_trans with Int.min_signed; auto.
+compute; congruence.
+apply Z.le_trans with Int.max_signed; auto.
+compute; congruence.
 
-Lemma typecheck_cmp_sound:
-forall op (Delta : tycontext) (rho : environ) (e1 e2 : expr) (t : type)
-   (CMP:  match op with Oeq | One | Olt | Ogt | Ole | Oge => True | _ => False end),
-   denote_tc_assert (typecheck_expr Delta e2) rho ->
-   denote_tc_assert (isBinOpResultType op e1 e2 t) rho ->
-   denote_tc_assert (typecheck_expr Delta e1) rho ->
-   typecheck_val (eval_expr e2 rho) (typeof e2) = true ->
-   typecheck_val (eval_expr e1 rho) (typeof e1) = true ->
-   typecheck_val
-     (eval_binop op (typeof e1) (typeof e2) (eval_expr e1 rho)
-        (eval_expr e2 rho)) t = true.
+assert (Int64.unsigned (Int64.repr (Int.unsigned i)) = Int64.unsigned (Int64.repr 0)) by (f_equal; auto).
+rewrite Int64.unsigned_repr in H.
+rewrite Int64.unsigned_repr in H.
+rewrite <- (Int.repr_unsigned i).
+rewrite H. reflexivity.
+split; compute; congruence. 
+pose proof (Int.unsigned_range i).
+clear - H1.
+destruct H1.
+split; auto.
+unfold Int64.max_unsigned.
+apply Z.le_trans with Int.modulus.
+omega.
+compute; congruence.
+Qed.
+
+Definition typecheck_numeric_val (v: val) (t: type) : Prop :=
+ match v,t with
+ | Vint _, Tint _ _ _ => True
+ | Vlong _, Tlong _ _ => True
+ | Vfloat _, Tfloat _ _ => True
+ | _, _ => False
+ end.
+
+
+
+Lemma typecheck_val_sem_cmp:
+ forall op v1 t1 v2 t2 i3 s3 a3,
+ typecheck_numeric_val v1 t1 ->
+ typecheck_numeric_val v2 t2 ->
+typecheck_val
+  (force_val
+     (sem_cmp op v1 t1 v2 t2 Mem.empty))
+  (Tint i3 s3 a3) = true.
 Proof.
-intros. rewrite den_isBinOpR in H0.
-destruct op; try (contradiction CMP);
-abstract(
-simpl in H0;
-intros; typecheck_sound_solver1 H0 e1 e2 t;
-unfold eval_binop; unfold sem_binary_operation, sem_cmp; simpl;
-remember (eval_expr e1 rho); destruct v; try solve[inv H3];
-remember (eval_expr e2 rho); destruct v; try solve[inv H2];
-try apply cmp_sound_aux;
-try (destruct H0; try contradiction;
-simpl in *; unfold is_true in *; rewrite H0; auto)).
+destruct op; intros;
+unfold sem_cmp, classify_cmp, typeconv,
+  sem_binarith, sem_cast, classify_cast;
+destruct v1; 
+  destruct t1 as [ | i1 s1 ? | i1 ? | i1 ? | | | | | | ];
+ try contradiction H;
+destruct v2; 
+  destruct t2 as [ | i2 s2 ? | i2 ? | i2 ? | | | | | | ];
+ try contradiction H0;
+ try destruct i1; try destruct s1; try destruct i2; try destruct s2;
+ simpl; 
+ try match goal with |- typecheck_val (Val.of_bool ?A) _ = _ =>
+  destruct A; reflexivity
+ end. 
 Qed.
 
-Lemma typecheck_sub_sound:
-forall (Delta : tycontext) (rho : environ) (e1 e2 : expr) (t : type),
-   denote_tc_assert (typecheck_expr Delta e2) rho ->
-   denote_tc_assert (isBinOpResultType Osub e1 e2 t) rho ->
-   typecheck_val (eval_expr e2 rho) (typeof e2) = true ->
-   typecheck_val (eval_expr e1 rho) (typeof e1) = true ->
-   typecheck_val
-     (eval_binop Osub (typeof e1) (typeof e2) (eval_expr e1 rho)
-        (eval_expr e2 rho)) t = true.
-Proof. 
-intros; typecheck_sound_solver1 H0 e1 e2 t;
-unfold tc_bool, eval_binop in *; simpl in *; unfold sem_sub; simpl;
-try (remember (Int.eq (Int.repr (sizeof t0)) Int.zero) as ez; destruct ez; simpl in *; auto);
- try (rewrite (Int.eq_false (Int.repr 1) Int.zero) in H0 by (intro Hx; inv Hx); simpl in H0);
-destruct (eval_expr e1 rho); inv H2; destruct (eval_expr e2 rho); inv H1;
- simpl in *; decompose [and] H0; try contradiction; auto;
- try (destruct (zeq b b0); inv H3; simpl; auto).
+Lemma typecheck_val_cmp_eqne_ip:
+ forall op v1 t1 v2 t0 a0 i2 s0 a1,
+ match op with Ceq => True | Cne => True | _ => False end ->
+ match v1,t1 with
+ | Vint i, Tint _ _ _ => Int.eq i Int.zero = true
+ | Vlong i, Tlong _ _ => Int.eq (Int.repr (Int64.unsigned i)) Int.zero = true
+ | _, _ => False
+ end ->
+ typecheck_val v2 (Tpointer t0 a0) = true ->
+typecheck_val
+  (force_val
+     (sem_cmp op v1 t1 v2 (Tpointer t0 a0) Mem.empty))
+  (Tint i2 s0 a1) = true.
+Proof.
+intros until 1; rename H into CMP; intros.
+ destruct op; try contradiction CMP; clear CMP;
+ destruct v1, t1; try contradiction H;
+ destruct v2; inv H0; try rewrite H2;
+ try destruct i0; destruct s; 
+unfold sem_cmp, classify_cmp, typeconv,
+  sem_binarith, sem_cast, classify_cast;
+ simpl; try rewrite H;
+ try reflexivity;
+ match goal with |- typecheck_val (Val.of_bool ?A) _ = _ =>
+  destruct A; reflexivity
+ end.
 Qed.
 
-Lemma typecheck_divmod_sound:
-forall op (Delta : tycontext) (rho : environ) (e1 e2 : expr) (t : type)
-   (OPER: match op with Odiv | Omod => True | _ => False end),
-   denote_tc_assert (typecheck_expr Delta e2) rho ->
-   denote_tc_assert (isBinOpResultType op e1 e2 t) rho ->
-    denote_tc_assert (typecheck_expr Delta e1) rho ->
-   typecheck_val (eval_expr e2 rho) (typeof e2) = true ->
-   typecheck_val (eval_expr e1 rho) (typeof e1) = true ->
-   typecheck_val
-     (eval_binop op (typeof e1) (typeof e2) (eval_expr e1 rho)
-        (eval_expr e2 rho)) t = true.
-Proof. 
-intros.
-destruct op; try contradiction;
-abstract (typecheck_sound_solver1 H0 e1 e2 t;
-(( destruct H0 as  [H0 H0']; hnf in H0,H0') ||
-(hnf in H0));
-destruct (eval_expr e1 rho); try contradiction;
-destruct (eval_expr e2 rho); try contradiction;
-unfold eval_binop, sem_binary_operation, sem_div, sem_mod;
-try (destruct (Int.eq i1 Int.zero); try (contradiction H0); simpl);
-try (destruct (Int.eq i0 (Int.repr Int.min_signed) && Int.eq i1 Int.mone);
-      inv H0');
- simpl; auto).
+Lemma typecheck_val_cmp_eqne_pi:
+ forall op v1 t1 v2 t0 a0 i2 s0 a1,
+ match op with Ceq => True | Cne => True | _ => False end ->
+ match v1,t1 with
+ | Vint i, Tint _ _ _ => Int.eq i Int.zero = true
+ | Vlong i, Tlong _ _ => Int.eq (Int.repr (Int64.unsigned i)) Int.zero = true
+ | _, _ => False
+ end ->
+ typecheck_val v2 (Tpointer t0 a0) = true ->
+typecheck_val
+  (force_val
+     (sem_cmp op v2 (Tpointer t0 a0) v1 t1 Mem.empty))
+  (Tint i2 s0 a1) = true.
+Proof.
+intros until 1; rename H into CMP; intros.
+ destruct op; try contradiction CMP; clear CMP;
+ destruct v1, t1; try contradiction H;
+ destruct v2; inv H0; try rewrite H2;
+ try destruct i0; destruct s; 
+unfold sem_cmp, classify_cmp, typeconv,
+  sem_binarith, sem_cast, classify_cast;
+ simpl; try rewrite H;
+ try reflexivity;
+ match goal with |- typecheck_val (Val.of_bool ?A) _ = _ =>
+  destruct A; reflexivity
+ end.
 Qed.
 
-Lemma typecheck_shift_sound:
-forall op (Delta : tycontext) (rho : environ) (e1 e2 : expr) (t : type)
-   (OPER: match op with Oshl | Oshr => True | _ => False end),
-   denote_tc_assert (typecheck_expr Delta e2) rho ->
-   denote_tc_assert (isBinOpResultType op e1 e2 t) rho ->
-   denote_tc_assert (typecheck_expr Delta e1) rho ->
-   typecheck_val (eval_expr e2 rho) (typeof e2) = true ->
-   typecheck_val (eval_expr e1 rho) (typeof e1) = true ->
-   typecheck_val
-     (eval_binop op (typeof e1) (typeof e2) (eval_expr e1 rho)
-        (eval_expr e2 rho)) t = true.
-Proof. 
-destruct op; try contradiction;
-abstract (
-intros; typecheck_sound_solver1 H0 e1 e2 t;
-unfold eval_binop; unfold sem_binary_operation, sem_shl, sem_shr; simpl;
-destruct (eval_expr e1 rho); inv H3;
-destruct (eval_expr e2 rho); inv H2;
-simpl; rewrite H0; reflexivity).
+Ltac sem_cmp_solver t1 t2 := 
+match t1 with 
+  | Tint ?i ?s _ => destruct i,s
+  | Tlong ?s _ => destruct s
+  | _ => idtac
+  end;
+  match t2 with 
+  | Tint ?i ?s _ => destruct i,s
+  | Tlong ?s _ => destruct s
+  | _ => idtac
+  end;
+  unfold sem_cmp; simpl;
+ repeat match goal with H: _ = true |- _ =>
+                try rewrite H; clear H
+            end;
+  try reflexivity;
+  match goal with 
+            |- typecheck_val (Val.of_bool ?A) _ = _ =>
+                destruct A; reflexivity
+            end.
+
+Lemma typecheck_sem_div_sound:
+ forall i i1 s1 a1 i0 i2 s2 a2 i3 s3 a3,
+ Int.eq i0 Int.zero = false ->
+ Int.eq i (Int.repr Int.min_signed) && Int.eq i0 Int.mone = false ->
+ typecheck_val
+  (force_val (sem_div (Vint i) (Tint i1 s1 a1) (Vint i0) (Tint i2 s2 a2))) (Tint i3 s3 a3) = true.
+Proof.
+ intros.
+ unfold sem_div, sem_binarith, sem_cast.
+ destruct i1,s1,i2,s2; simpl; rewrite H; try rewrite H0; reflexivity.
+Qed.
+
+Lemma typecheck_sem_mod_sound:
+ forall i i1 s1 a1 i0 i2 s2 a2 i3 s3 a3,
+ Int.eq i0 Int.zero = false ->
+ Int.eq i (Int.repr Int.min_signed) && Int.eq i0 Int.mone = false ->
+ typecheck_val
+  (force_val (sem_mod (Vint i) (Tint i1 s1 a1) (Vint i0) (Tint i2 s2 a2))) (Tint i3 s3 a3) = true.
+Proof.
+ intros.
+ unfold sem_mod, sem_binarith, sem_cast.
+ destruct i1,s1,i2,s2; simpl; rewrite H; try rewrite H0; reflexivity.
 Qed.
 
 
-
-Ltac typecheck_sound_solver Delta rho e1 e2 t :=
- match goal with
- | H: denote_tc_assert (typecheck_expr Delta e2) rho,
-   H0: denote_tc_assert (isBinOpResultType _ e1 e2 t) rho,
-   H1: typecheck_val (eval_expr e2 rho) (typeof e2) = true,
-   H2: typecheck_val (eval_expr e1 rho) (typeof e1) = true |- _ =>
- typecheck_sound_solver1 H0 e1 e2 t;
-try solve [destruct (eval_expr e1 rho); inv H2;
-               destruct (eval_expr e2 rho); inv H1;
-               try (contradiction H0);
-               simpl; auto]
-end.
+Ltac crunch := 
+repeat (
+ unfold is_true in *; simpl;
+ match goal with 
+  | H: ?f _ = ?f _ |- _ => inv H
+  | |- _ => first [contradiction | discriminate | reflexivity
+                         | rewrite or_False in * | rewrite False_or in * | rewrite zeq_true ]
+  | H: denote_tc_assert' (tc_bool ?A _) _ |- _ => 
+     destruct A eqn:?; try contradiction H; clear H
+  | H: denote_tc_assert' (tc_andp' _ _) _ |- _ => 
+     apply denote_tc_assert'_andp'_e in H; destruct H
+  | H: denote_tc_assert' (tc_orp' _ _) _ |- _ => hnf in H
+ | H: denote_tc_assert' (tc_isptr _) _ |- _ => hnf in H
+ | H: denote_tc_assert' (tc_ilt _ _) _ |- _ => hnf in H
+ | H: denote_tc_assert' (tc_iszero' _) _ |- _ => hnf in H
+ | H: denote_tc_assert' (tc_nonzero _) _ |- _ => hnf in H
+ | H: denote_tc_assert' (tc_nodivover _ _) _ |- _ => hnf in H
+ | H: denote_tc_assert' (tc_samebase _ _) _ |- _ => hnf in H
+ | H: denote_tc_iszero _ |- _ => hnf in H
+  | H: ?A=true |- _ => rewrite H; simpl
+  | H: ?A=false |- _ => rewrite H; simpl
+  | H: negb ?A = true |- _ => destruct A eqn:?; inv H; simpl; auto
+  | H: if negb ?A then True else False |- _ => 
+           destruct A eqn:?; try contradiction H; clear H; simpl; auto 
+ | H: denote_tc_assert' (match ?A with _ => _ end) _ |- _ => 
+          first [is_var A; destruct A 
+                 | let J := fresh in destruct A eqn:J; move J before H]
+  | H: match ?A with _ => _ end = _ |- _ => 
+          first [is_var A; destruct A 
+                 | let J := fresh in destruct A eqn:?; move J before H]
+  | H: is_int_type ?t = true |- _ => destruct t; inv H 
+  | H: is_long_type ?t = true |- _ => destruct t; inv H 
+  | H: is_float_type ?t = true |- _ => destruct t; inv H
+  | H: is_pointer_type ?t = true |- _ => destruct t; inv H  
+  | H: andb _ _ = true |- _ => apply -> andb_true_iff in H; destruct H
+  | H: proj_sumbool (zeq ?b ?b') = true |- _ =>  destruct (zeq b b'); inv H
+  | |- typecheck_val (Val.of_bool ?A) _ = _ => destruct A
+  end).
 
 Lemma typecheck_binop_sound:
-forall (Delta : tycontext) (rho : environ) (b : binary_operation)
-  (e1 e2 : expr) (t : type),
-denote_tc_assert (typecheck_expr Delta (Ebinop b e1 e2 t)) rho ->
-(denote_tc_assert (typecheck_expr Delta e1) rho ->
- typecheck_val (eval_expr e1 rho) (typeof e1) = true) ->
-(denote_tc_assert (typecheck_expr Delta e2) rho ->
- typecheck_val (eval_expr e2 rho) (typeof e2) = true) ->
-typecheck_val (eval_expr (Ebinop b e1 e2 t) rho) (typeof (Ebinop b e1 e2 t)) =
-true.
-Proof. 
-intros. simpl in *.  rewrite tc_andp_sound in H. 
-simpl in *. super_unfold_lift; rewrite tc_andp_sound in H. 
-simpl in *. super_unfold_lift; intuition.  
-destruct b;
-try (eapply typecheck_sub_sound; eauto);
-try solve [eapply typecheck_divmod_sound; simpl; eauto];
-try solve [eapply typecheck_shift_sound; simpl; eauto];
-try solve [eapply typecheck_cmp_sound; simpl; eauto];
-clear H4; abstract (typecheck_sound_solver Delta rho e1 e2 t).
+forall op (Delta : tycontext) (rho : environ) (e1 e2 : expr) (t : type)
+   (IBR: denote_tc_assert (isBinOpResultType op e1 e2 t) rho)
+   (TV2: typecheck_val (eval_expr e2 rho) (typeof e2) = true)
+   (TV1: typecheck_val (eval_expr e1 rho) (typeof e1) = true),
+   typecheck_val
+     (eval_binop op (typeof e1) (typeof e2) (eval_expr e1 rho)
+        (eval_expr e2 rho)) t = true.
+Proof.
+intros; destruct op;
+abstract (
+rewrite den_isBinOpR in IBR; simpl in IBR;
+ let E1 := fresh "E1" in let E2 := fresh "E2" in 
+ destruct (typeof e1) as [ | i1 s1 ? | s1 ? | i1 ? | | | | | | ];
+ destruct (eval_expr e1 rho) eqn:E1; inv TV1;
+ destruct (typeof e2) as [ | i2 s2 ? | s2 ? | i2 ? | | | | | | ];
+ try solve [inv IBR];
+ destruct (eval_expr e2 rho) eqn:E2; inv TV2;
+unfold eval_binop, sem_binary_operation;
+unfold classify_cmp',classify_add',classify_sub',classify_shift',stupid_typeconv,
+  binarithType, classify_binarith in IBR;
+ rewrite <- denote_tc_assert'_eq in IBR;
+crunch;
+try rewrite E1 in *; 
+try rewrite E2 in *; 
+simpl in *; crunch;
+try match goal with
+| |- _ => first [simple apply typecheck_val_sem_cmp; apply I
+                         |  simple apply typecheck_sem_div_sound; assumption 
+                         |  simple apply typecheck_sem_mod_sound; assumption]
+| |- context [sem_add] =>
+  unfold sem_add; rewrite classify_add_eq; unfold classify_add', stupid_typeconv; 
+  reflexivity
+ | |- typecheck_val (force_val ((sem_cmp _ _ ?t1 _ ?t2) _)) _ = true =>
+        sem_cmp_solver t1 t2
+| |- context [sem_sub] =>
+     unfold sem_sub; rewrite classify_sub_eq; unfold classify_sub', stupid_typeconv; 
+     try rewrite zeq_true;
+     try match goal with H: Int.eq _ Int.zero = false |- _ => rewrite H end;
+    reflexivity
+ | H: Int.eq ?i0 Int.zero = false |- typecheck_val  (force_val  (_ _ _ (Vint ?i0) _)) _ = true =>
+       unfold sem_div, sem_mod, sem_binarith, sem_cast;
+       simpl; (rewrite H || rewrite cast_int_long_nonzero by assumption); 
+       reflexivity
+ | H: Int.ltu _ Int.iwordsize = true |- typecheck_val  (force_val  (_ _ _ (Vint ?i0) _)) _ = true =>
+       unfold sem_shl, sem_shr, sem_shift;
+     rewrite classify_shift_eq; unfold classify_shift', stupid_typeconv;
+  simpl; rewrite H; reflexivity
+end).
 Qed.
-
-
