Makefile
@@ -58,15 +58,16 @@ SEPCOMP_FILES= \
   mem_interpolation_EE.v mem_interpolation_EI.v \
   mem_interpolation_IE.v mem_interpolation_II.v \
   mem_interpolation_proofs.v \
-  core_semantics.v 
+  core_semantics.v \
+ forward_simulations.v rg_forward_simulations.v \
+  extension.v extension_proof.v 
 #  compile_safe.v core_semantics_lemmas.v \
-  forward_simulations.v rg_forward_simulations.v \
-  forward_simulations_lemmas.v \
-  extension.v extension_safety.v extension_simulations.v \
-  extension_proof_safety.v extension_proof.v \
-  null_extension.v fs_extension.v linking_extension.v trace_extension.v \
-  mem_interpolants.v compiler_correctness_trans.v \
-  compcert_compiler_correctness.v RG_interpolants.v rgsim.v
+#  forward_simulations_lemmas.v \
+#   extension_safety.v extension_simulations.v \
+#  extension_proof_safety.v 
+#  null_extension.v fs_extension.v linking_extension.v trace_extension.v \
+#  mem_interpolants.v compiler_correctness_trans.v \
+#  compcert_compiler_correctness.v RG_interpolants.v rgsim.v
 
 VERIC_FILES= \
   base.v rmaps.v rmaps_lemmas.v compcert_rmaps.v \
